fix and simplify thetac proof

Clean/Gadgets/Keccak/ThetaC.lean
@@ -11,12 +11,9 @@ variable [p_large_enough: Fact (p > 512)]
 
 open FieldUtils (mod_256 floordiv)
 open Xor (xor_u64)
-open Clean.Gadgets.Keccak256 (KeccakState)
+open Clean.Gadgets.Keccak256 (KeccakState KeccakSlice)
 
-@[reducible] def Outputs := ProvableVector U64 5
--- note: `reducible` is needed for type class inference, i.e. `ProvableType KeccakState`
-
-def theta_c (state : Var KeccakState (F p)) : Circuit (F p) (Var Outputs (F p)) := do
+def theta_c (state : Var KeccakState (F p)) : Circuit (F p) (Var KeccakSlice (F p)) := do
   -- TODO would be nice to have a for loop of length 5 here
   let c0 ← subcircuit Gadgets.Xor.circuit ⟨(state.get 0), (state.get 1)⟩
   let c0 ← subcircuit Gadgets.Xor.circuit ⟨c0, (state.get 2)⟩
@@ -44,23 +41,15 @@ def theta_c (state : Var KeccakState (F p)) : Circuit (F p) (Var Outputs (F p)) 
   let c4 ← subcircuit Gadgets.Xor.circuit ⟨c4, (state.get 24)⟩
   return #v[c0, c1, c2, c3, c4]
 
-def assumptions (state : KeccakState (F p)) : Prop :=
-  ∀ i : Fin 25, state[i].is_normalized
+def assumptions (state : KeccakState (F p)) := state.is_normalized
 
-def spec (state : KeccakState (F p)) (out: Outputs (F p)) : Prop :=
-  let h_norm := out[0].is_normalized ∧ out[1].is_normalized ∧
-             out[2].is_normalized ∧ out[3].is_normalized ∧ out[4].is_normalized
-
-  let state_u64 := state.map (fun x => x.value)
-  let out_u64 := out.map (fun x => x.value)
-
-  let state' := Clean.Gadgets.Keccak256.theta_c state_u64
-
-  h_norm ∧ state' = out_u64
+def spec (state : KeccakState (F p)) (out: KeccakSlice (F p)) :=
+  out.is_normalized
+  ∧ out.value = Clean.Gadgets.Keccak256.theta_c state.value
 
 -- #eval! theta_c (p:=p_babybear) default |>.operations.local_length
 -- #eval! theta_c (p:=p_babybear) default |>.output
-instance elaborated : ElaboratedCircuit (F p) KeccakState (Var Outputs (F p)) where
+instance elaborated : ElaboratedCircuit (F p) KeccakState (Var KeccakSlice (F p)) where
   main := theta_c
   local_length _ := 160
   output _ i0 := #v[
@@ -73,18 +62,16 @@ instance elaborated : ElaboratedCircuit (F p) KeccakState (Var Outputs (F p)) wh
 
 theorem soundness : Soundness (F p) assumptions spec := by
   intro i0 env state_var state h_input state_norm h_holds
-  simp only [circuit_norm] at h_input
-  dsimp only [assumptions] at state_norm
-  dsimp only [circuit_norm, theta_c, Xor.circuit] at h_holds
-  simp only [circuit_norm, subcircuit_norm] at h_holds
-  dsimp only [Xor.assumptions, Xor.spec] at h_holds
-  simp [add_assoc, and_assoc, -Fin.val_zero, -Fin.val_one', -Fin.val_one, -Fin.val_two] at h_holds
+  simp only [circuit_norm, subcircuit_norm, assumptions,
+    theta_c, Xor.circuit, Xor.assumptions, Xor.spec] at *
+  simp only [and_imp, and_assoc, add_assoc, Nat.reduceAdd] at h_holds
 
   have s (i : Fin 25) : eval env (state_var[i.val]) = state[i.val] := by
     rw [←h_input, Vector.getElem_map]
-
   simp only [s] at h_holds
-  simp [circuit_norm, spec]
+  simp only [circuit_norm, spec, KeccakSlice.is_normalized_iff,
+    KeccakSlice.value, KeccakState.value,
+    Clean.Gadgets.Keccak256.theta_c, Clean.Gadgets.Keccak256.xor_u64]
 
   repeat
     first
@@ -97,11 +84,9 @@ theorem soundness : Soundness (F p) assumptions spec := by
     rw [xor02, xor01, xor00] at xor0
     clear h00 h01 h02 h03 norm00 norm01 norm02 xor00 xor01 xor02
 
+  simp [*]
 
-  simp [Clean.Gadgets.Keccak256.theta_c, Clean.Gadgets.Keccak256.xor_u64, spec]
-  simp only [true_and, Fin.isValue, Fin.val_zero, Fin.val_one, Fin.val_two, *]
-
-theorem completeness : Completeness (F p) Outputs assumptions := by
+theorem completeness : Completeness (F p) KeccakSlice assumptions := by
   intro i0 env state_var h_env state h_input h_assumptions
   simp only [circuit_norm] at h_input
   dsimp only [circuit_norm, theta_c, Xor.circuit]
@@ -116,7 +101,7 @@ theorem completeness : Completeness (F p) Outputs assumptions := by
 
   sorry
 
-def circuit : FormalCircuit (F p) KeccakState Outputs := {
+def circuit : FormalCircuit (F p) KeccakState KeccakSlice := {
   elaborated with
   main := theta_c
   assumptions
